{
 "cells": [
  {
   "cell_type": "markdown",
   "metadata": {},
   "source": [
    "---\n",
    "\n",
    "(latex macros)\n",
    "$\n",
    "\\def\\bba#1\\eea{\\begin{align}#1\\end{align}}\n",
    "\\def\\bbm#1\\eem{\\begin{matrix}#1\\end{matrix}}\n",
    "\\newcommand{\\tt}[0]{\\text}\n",
    "\\newcommand{\\pp}[0]{\\partial}\n",
    "\\newcommand{\\ll}[0]{\\left}\n",
    "\\newcommand{\\rr}[0]{\\right}\n",
    "\\newcommand{\\ffbb}[0]{\\mathbb}\n",
    "\\newcommand{\\Re}[1]{\\text{Re}\\left(#1\\right)}\n",
    "\\newcommand{\\Im}[1]{\\text{Im}\\left(#1\\right)}\n",
    "\\newcommand{\\iprod}[2]{\\left< #1, #2 \\right>}\n",
    "$\n",
    "\n",
    "---"
   ]
  },
  {
   "cell_type": "markdown",
   "metadata": {},
   "source": [
    "## SOR method\n",
    "\n",
    "\n",
    "### Def. 1\n",
    "\n",
    "Given $A \\in \\ffbb{C}^{n \\times n}$, we write $A = D + L + U$ where each D/L/U has diagonal/lower/upper parts of A.\n",
    "\n",
    "Define ***w-SOR operator*** $x \\mapsto x''$  by:\n",
    "\n",
    "$~~\n",
    "\\bba\n",
    "D x' = - L x'' - U x + b \\\\\n",
    "x'' = (1 - w) x + w x',\n",
    "\\eea\n",
    "$\n",
    "\n",
    "i.e.\n",
    "\n",
    "$~~\n",
    "\\bba\n",
    "& D x'' = (1 - w) D x + w D x' = (1 - w) D x + w (- L x'' - U x + b) \\\\\n",
    "& \\begin{aligned}\n",
    "    \\iff\n",
    "        \\ll( \\frac{1}{w} D + L \\rr) x''\n",
    "            &= (\\frac{1 - w}{w} D - U) x + b\n",
    "             = - \\ll( \\ll( 1 - \\frac{1}{w} \\rr) D + U \\rr) x + b \\\\\n",
    "            &= - \\ll(A - \\ll( \\frac{1}{w} D + L \\rr) \\rr) x + b.\n",
    "  \\end{aligned}\n",
    "\\eea\n",
    "$\n",
    "\n",
    "When $w = 1$, it produces ***Gauss-Seidel operator***, which is defined by:\n",
    "\n",
    "$~~ (D + L) x' + U x = b ~~$ i.e. $~~ x' = (D + L)^{-1}(- U x + b)$."
   ]
  },
  {
   "cell_type": "markdown",
   "metadata": {},
   "source": [
    "### Prop. 2.\n",
    "\n",
    "(Cf. Stoer, Bulirsch Thm. 8.3.7.)\n",
    "\n",
    "Given\n",
    "\n",
    "- $A$ : positive definite,\n",
    "- $w \\in (0, 2)$,\n",
    "- $B \\equiv \\frac{1}{w} D + L$,\n",
    "- $H \\equiv B^{-1}(B - A) = I - B^{-1} A$,\n",
    "\n",
    "then $\\rho(H) \\lt 1$.\n",
    "\n",
    "***Proof***\n",
    "\n",
    "First we (magically) find that:\n",
    "\n",
    "$~~\n",
    "\\bba\n",
    "H &= I - B^{-1} A  \\\\\n",
    "    &= (A^{-1} B - I) B^{-1} A  \\\\\n",
    "    &= (A^{-1} B - I) (A^{-1} B)^{-1} \\\\\n",
    "    &= (2 A^{-1} B - 2 I) (2 A^{-1} B)^{-1} \\\\    \n",
    "    &= \\ll( (2 A^{-1} B - I) - I \\rr) ((2 A^{-1} B - I) + I)^{-1},\n",
    "\\eea\n",
    "$\n",
    "\n",
    "thus, writing $Q = 2 A^{-1} B - I$, we have $H = (Q - I) (Q + I)^{-1}$.\n",
    "\n",
    "Now, given eigen value $\\mu$ and eigen vector $x$ of $H$ as in $H x = \\mu x$,\n",
    "we define $y = (R + I)^{-1} x$ and we see:\n",
    "\n",
    "$~~\n",
    "\\bba\n",
    "H x = \\mu x\n",
    "    &\\iff (Q - I) \\ll( (Q + I)^{-1} x \\rr) = \\mu (Q + I) \\ll( (Q + I)^{-1} x \\rr) \\\\\n",
    "    &\\iff Qy - y = \\mu Q y + \\mu y \\\\\n",
    "    &\\iff Q y = \\frac{1 + \\mu}{1 - \\mu} y.\n",
    "\\eea\n",
    "$\n",
    "\n",
    "Here, we observe:\n",
    "\n",
    "$~~\n",
    "\\bba\n",
    "\\frac{1 + \\mu}{1 - \\mu}\n",
    "    &= \\frac{(1 + \\mu)(1 - \\mu^\\dagger)}{|1 - \\mu|^2}\n",
    "     = \\frac{1 + i \\Im{\\mu} - |\\mu|^2}{|1 - \\mu|^2} \\\\\n",
    "\\Re{\\frac{1 + \\mu}{1 - \\mu}}\n",
    "    &= \\frac{1 - |\\mu|^2}{|1 - \\mu|^2}.\n",
    "\\eea\n",
    "$\n",
    "\n",
    "Thus, \n",
    "\n",
    "$~~\n",
    "\\Re{\\frac{1 + \\mu}{1 - \\mu}} > 0  \\iff  1 - |\\mu|^2 > 0  \\iff |\\mu| < 1,\n",
    "$\n",
    "\n",
    "so, to our goal, it's suffices to show $\\Re{\\tt{eigen value of $Q$}} > 0$.\n",
    "\n",
    "Proving this, we take $Q y = (2 A^{-1} B - I) y = \\lambda y$, then we see:\n",
    "\n",
    "$~~\n",
    "\\bba\n",
    "&(2 A^{-1} B - I) y = \\lambda y  \\\\\n",
    "&\\iff A^{-1} (2 B - A) y = \\lambda y  \\\\\n",
    "&\\iff (2 B - A) y = \\lambda A y \\\\\n",
    "&\\implies\n",
    "    \\begin{cases}\n",
    "        \\iprod{y}{(2 B - A) y}         &= \\iprod{y}{\\lambda A y} \\\\\n",
    "        \\iprod{y}{(2 B - A)^\\dagger y} &= \\iprod{y}{\\lambda^\\dagger A^\\dagger y}\n",
    "    \\end{cases} \\\\\n",
    "&\\iff\n",
    "    \\begin{cases}\n",
    "        \\iprod{y}{(2 B - A) y}         &= \\iprod{y}{\\lambda A y} \\\\\n",
    "        \\iprod{y}{(2 B^\\dagger - A) y} &= \\iprod{y}{\\lambda^\\dagger A y}\n",
    "    \\end{cases} ~~~(\\tt{since $A$ : Hermittian}) \\\\\n",
    "&\\implies\n",
    "    \\iprod{y}{\\ll( 2 (B + B^\\dagger) - 2 A \\rr) y} = (\\lambda + \\lambda^\\dagger) \\iprod{y}{A y}\n",
    "    ~~~(\\tt{adding above two equations}) \\\\\n",
    "&\\implies\n",
    "    \\iprod{y}{\\ll((B + B^\\dagger) - A \\rr) y} = \\Re{\\lambda}\\iprod{y}{A y}\n",
    "\\eea\n",
    "$\n",
    "\n",
    "But here, $(B + B^\\dagger) - A = \\frac{2}{w} D + L + L^\\dagger - A = \\ll(\\frac{2}{w} - 1\\rr) D$ : positive definite.\n",
    "\n",
    "Thus, we obtain $\\Re{\\lambda} > 0$."
   ]
  }
 ],
 "metadata": {
  "kernelspec": {
   "display_name": "Python 3",
   "language": "python",
   "name": "python3"
  },
  "language_info": {
   "codemirror_mode": {
    "name": "ipython",
    "version": 3
   },
   "file_extension": ".py",
   "mimetype": "text/x-python",
   "name": "python",
   "nbconvert_exporter": "python",
   "pygments_lexer": "ipython3",
   "version": "3.8.2"
  }
 },
 "nbformat": 4,
 "nbformat_minor": 4
}
