{
 "cells": [
  {
   "cell_type": "markdown",
   "metadata": {},
   "source": [
    "---\n",
    "\n",
    "(latex macro definitions)\n",
    "\n",
    "$\n",
    "\\def\\Mm#1\\mm{\\begin{matrix}#1\\end{matrix}}\n",
    "\\def\\Mmp#1\\mmp{\\begin{pmatrix}#1\\end{pmatrix}}\n",
    "\\def\\Mmv#1\\mmv{\\begin{vmatrix}#1\\end{vmatrix}}\n",
    "\\def\\Aa#1\\aa{\\begin{align}#1\\end{align}}\n",
    "\\def\\Cc#1\\cc{\\begin{cases}#1\\end{cases}}\n",
    "\\newcommand{\\tt}[0]{\\text}\n",
    "\\newcommand{\\ll}[0]{\\left}\n",
    "\\newcommand{\\rr}[0]{\\right}\n",
    "\\newcommand{\\pp}[0]{\\partial}\n",
    "\\newcommand{\\eqarrow}[0]{\\Leftrightarrow}\n",
    "$\n",
    "\n",
    "---"
   ]
  },
  {
   "cell_type": "markdown",
   "metadata": {},
   "source": [
    "## Symplectic map and generating function\n",
    "\n",
    "(note that we order coordinates in $R^{2n}$ by $(p_1, .., p_n, q_1, .., q_n)$.)\n",
    "\n",
    "### Def. 1\n",
    "\n",
    "$\n",
    "\\phi : R^{2n} \\to R^{2n} : \\tt{symplectic map}\n",
    "\\eqarrow\n",
    "(D\\phi)^T J D\\phi = J\n",
    "$\n",
    "\n",
    "where \n",
    "\n",
    "- $D\\phi$ : Jacobian of $\\phi$,\n",
    "- $J = \\Mmp 0 & I \\\\ -I & 0 \\mmp$.\n",
    "\n",
    "\n",
    "### Prop. 2\n",
    "\n",
    "$\n",
    "\\phi : \\tt{symplectic map}\n",
    "\\eqarrow\n",
    "\\phi^{*} (dp_i \\wedge dq_i) = dp_i \\wedge dq_i\n",
    "$\n",
    "\n",
    "(note that \"$dp_i \\wedge dq_i$\" denotes $\\sum_i dp_i \\wedge dq_i$)\n",
    "\n",
    "***Proof***\n",
    "\n",
    "We obtain result from:\n",
    "\n",
    "$\n",
    "\\Aa\n",
    "(dp_i \\wedge dq_i) (u, v)\n",
    "    = \\sum_i u_{p_i} v_{q_i} - u_{q_i} v_{p_i}\n",
    "    =  u^T J v,\n",
    "\\aa\n",
    "$\n",
    "\n",
    "and,\n",
    "\n",
    "$\n",
    "\\Aa\n",
    "(\\phi^{*} (dp_i \\wedge dq_i)) (u, v)\n",
    "    = (dp_i \\wedge dq_i) (D\\phi(u), D\\phi(v))\n",
    "    = (D\\phi(u))^T J D\\phi(v).\n",
    "\\aa\n",
    "$"
   ]
  },
  {
   "cell_type": "markdown",
   "metadata": {},
   "source": [
    "### Prop. 3\n",
    "\n",
    "$\n",
    "\\Aa\n",
    "\\phi : \\tt{symplectic map}\n",
    "&\\eqarrow\n",
    "    \\phi^{*}(p_i dq_i) - p_i dq_i = dS \\quad \\tt{for some S} \\\\\n",
    "&\\eqarrow\n",
    "    \\phi^{*}(q_i dp_i) + p_i dq_i = dS \\quad \\tt{for some S} \\\\\n",
    "&\\eqarrow\n",
    "    \\phi^{*}(p_i dq_i) + q_i dp_i = dS \\quad \\tt{for some S}. \\\\\n",
    "\\aa\n",
    "$\n",
    "\n",
    "\n",
    "***Proof***\n",
    "\n",
    "Noting:\n",
    "\n",
    "$\n",
    "\\Aa\n",
    "dp_i \\wedge dq_i           &= d(p_i dq_i) = - d(q_i dp_i) \\\\\n",
    "\\phi^{*}(dp_i \\wedge dq_i) &= d(\\phi^{*}(p_i dq_i)) = - d(\\phi^{*}(q_i dp_i)),\n",
    "\\aa\n",
    "$\n",
    "\n",
    "we have:\n",
    "\n",
    "$\n",
    "\\Aa\n",
    "\\phi^{*}(dp_i \\wedge dq_i) = dp_i \\wedge dq_i\n",
    "    &\\eqarrow\n",
    "        \\phi^{*}(dp_i \\wedge dq_i) - dp_i \\wedge dq_i = 0 \\\\\n",
    "    &\\eqarrow\n",
    "        \\phi^{*}(p_i dq_i) - p_i dq_i : \\tt{exact} \\\\\n",
    "    &\\eqarrow\n",
    "        \\phi^{*}(q_i dp_i) + p_i dq_i : \\tt{exact} \\\\\n",
    "    &\\eqarrow\n",
    "        \\phi^{*}(p_i dq_i) + q_i dp_i : \\tt{exact}.   \n",
    "\\aa\n",
    "$\n",
    "\n",
    "Then, \"closed\" $\\eqarrow$ \"exact\" follows from Poincare's lemma."
   ]
  },
  {
   "cell_type": "markdown",
   "metadata": {},
   "source": [
    "### Prop. 4\n",
    "\n",
    "We write $\\phi(p, q) = (\\hat{p}(p, q), \\hat{q}(p, q))$.\n",
    "\n",
    "We assume $\\exists S : R^{2n} \\to R$ s.t.\n",
    "\n",
    "$\n",
    "\\Cc\\Aa\n",
    "            p &= \\pp_{q} S(\\hat{p}(p, q), q)  \\\\\n",
    "\\hat{q}(p, q) &= \\pp_{\\hat{p}} S(\\hat{p}(p, q), q).\n",
    "\\aa\\cc\n",
    "$\n",
    "\n",
    "Then, $\\phi$ : symplectic map.\n",
    "\n",
    "\n",
    "***Proof***\n",
    "\n",
    "We define $\\psi : R^{2n} \\to R^{2n}$ s.t.\n",
    "\n",
    "$\n",
    "\\psi(p, q) = (\\hat{p}(p, q), q).\n",
    "$\n",
    "\n",
    "Then,\n",
    "\n",
    "$\n",
    "\\Aa\n",
    "d(\\psi^*(S))\n",
    "    &= \\psi^*(dS) \\\\\n",
    "    &= \\psi^*(\\pp_{p_i} S(p, q) dp_i + \\pp_{q_i} S(p, q) dq_i) \\\\\n",
    "    &= \\pp_{\\hat{p_i}} S(\\hat{p}, q) d(\\hat{p}_i) + \\pp_{q_i} S(\\hat{p}, q) dq_i \\\\\n",
    "    &= \\pp_{\\hat{p_i}} S(\\hat{p}, q) d(\\hat{p}_i) + \\pp_{q_i} S(\\hat{p}, q) dq_i \\\\    \n",
    "    &= \\hat{q}_i d(\\hat{p}_i) + p_i dq_i. \\\\\n",
    "\\aa\n",
    "$\n",
    "\n",
    "Thus, our result follows from \"Prof. 3\"."
   ]
  },
  {
   "cell_type": "markdown",
   "metadata": {},
   "source": [
    "---"
   ]
  },
  {
   "cell_type": "markdown",
   "metadata": {},
   "source": [
    "## Verlet integration\n",
    "\n",
    "\n",
    "### Def. 1\n",
    "\n",
    "Given a differential equation of the form:\n",
    "\n",
    "$\n",
    "\\Aa\n",
    "\\pp_t x(t)\n",
    "    = G(x(t)),\n",
    "\\aa\n",
    "$\n",
    "\n",
    "by separting components by $x = \\Mmp p \\\\ q \\mmp$, we also write:\n",
    "\n",
    "$\n",
    "\\Aa\n",
    "\\pp_t \\Mmp p \\\\ q \\mmp\n",
    "    = \\Mmp G_p(p, q) \\\\ G_q(p, q) \\mmp,\n",
    "\\aa\n",
    "$\n",
    "\n",
    "(note that $G_p$ denotes p-components of vector $G$ and it's not partial derivative,)\n",
    "\n",
    "then, we define ***p-implicit method*** and ***q-implicit method*** as follows:\n",
    "\n",
    "- p-implicit method:\n",
    "\n",
    "$\n",
    "\\Cc\\Aa\n",
    "p_1 &= p_0 + h G_p(p_1, q_0) \\\\\n",
    "q_1 &= q_0 + h G_q(p_1, q_0),\n",
    "\\aa\\cc\n",
    "$\n",
    "\n",
    "\n",
    "- q-implicit method:\n",
    "\n",
    "$\n",
    "\\Cc\\Aa\n",
    "p_1 &= p_0 + h G_p(p_0, q_1) \\\\\n",
    "q_1 &= q_0 + h G_q(p_0, q_1),\n",
    "\\aa\\cc\n",
    "$"
   ]
  },
  {
   "cell_type": "markdown",
   "metadata": {},
   "source": [
    "We also define ***pq-implicit method*** and ***qp-implicit method***\n",
    "by alternating above methods in two steps.\n",
    "\n",
    "- pq-implicit method\n",
    "\n",
    "$\n",
    "\\Cc\\Aa\n",
    "p_1 &= p_0 + h G_p(p_1, q_0) \\\\\n",
    "q_1 &= q_0 + h G_q(p_1, q_0) \\\\\n",
    "p_2 &= p_1 + h G_p(p_1, q_2) \\\\\n",
    "q_2 &= q_1 + h G_q(p_1, q_2),\n",
    "\\aa\\cc\n",
    "$\n",
    "\n",
    "- qp-implicit method\n",
    "\n",
    "$\n",
    "\\Cc\\Aa\n",
    "p_1 &= p_0 + h G_p(p_0, q_1) \\\\\n",
    "q_1 &= q_0 + h G_q(p_0, q_1) \\\\\n",
    "p_2 &= p_1 + h G_p(p_2, q_1) \\\\\n",
    "q_2 &= q_1 + h G_q(p_2, q_1),\n",
    "\\aa\\cc\n",
    "$"
   ]
  },
  {
   "cell_type": "markdown",
   "metadata": {},
   "source": [
    "### Prop. 2.\n",
    "\n",
    "For p-implicit and q-implicit method, we have:\n",
    "\n",
    "$\n",
    "x(h) - x_1 = O(h^2).\n",
    "$\n",
    "\n",
    "(aka. convergence of 1st order.)\n",
    "\n",
    "***Proof***\n",
    "\n",
    "Here, we only show the proof for p-implicit method. \n",
    "\n",
    "Noting:\n",
    "\n",
    "$\n",
    "\\Aa\n",
    "G_p(p_1, q_0)\n",
    "    &= G_p(p_0 + h G_p(p_1, q_0), q_0) \\\\\n",
    "    &= G_p(p_0, q_0) + O((h G_p(p_1, q_0))) \\\\\n",
    "    &= \\dot{p}_0 + O(h),    \n",
    "\\aa\n",
    "$\n",
    "\n",
    "thus,\n",
    "\n",
    "$\n",
    "\\Aa\n",
    "p_1 &= p_0 + h G_p(p_1, q_0) = p_0 + h \\dot{p}_0 + O(h^2)\n",
    "\\\\\n",
    "q_1 &= q_0 + h G_q(p_1, q_0) = q_0 + h \\dot{q}_0 + O(h^2).\n",
    "\\aa\n",
    "$\n",
    "\n",
    "i.e. $x_1 = x_0 + h \\dot{x}_0 + O(h^2)$.\n",
    "\n",
    "On the other hand, by Taylor expansion, we have $x(h) = x(0) + h \\dot{x}(0) + O(h^2)$, so our result follows."
   ]
  },
  {
   "cell_type": "markdown",
   "metadata": {},
   "source": [
    "### Prop. 3.\n",
    "\n",
    "For pq-implicit method and qp-implicit method, we have:\n",
    "\n",
    "$\n",
    "x(2h) - x_2 = O(h^3).\n",
    "$\n",
    "\n",
    "(aka. convergence of 2nd order.)\n",
    "\n",
    "***Proof***\n",
    "\n",
    "Here, we only show the proof of qp-implicit method.\n",
    "\n",
    "First, by Taylor expansion around $t = h$, we have:\n",
    "\n",
    "$\n",
    "x(2h) - x(0) = 2 h \\dot{x}(h) + O(h^3).\n",
    "$\n",
    "\n",
    "On the other hand, we see\n",
    "\n",
    "$\n",
    "\\Aa\n",
    "p_2 - p_0 &= h ( G_p(p_0, q_1) + G_p(p_2, q_1) ) \\\\\n",
    "q_2 - q_0 &= h ( G_q(p_0, q_1) + G_q(p_2, q_1) ),\n",
    "\\aa\n",
    "$\n",
    "\n",
    "and,\n",
    "\n",
    "$\n",
    "\\Aa\n",
    "G_p(p_0, q_1) + G_p(p_2, q_1)\n",
    "    &= G_p(p_1 - h G_p(p_0, q_1), q_1) + G_p(p_1 + h G_p(p_2, q_1), q_1) \\\\\n",
    "    &= 2 G_p(p_1, q_1) + h \\pp_p G_p(p_1, q_1) (G_p(p_2, q_1) - G_p(p_0, q_1)) + O(h^2),\n",
    "\\aa\n",
    "$\n",
    "\n",
    "and,\n",
    "\n",
    "$\n",
    "\\Aa\n",
    "G_p(p_2, q_1) - G_p(p_0, q_1)\n",
    "    &= G_p(p_1 + h G_p(p_2, q_1), q_1) - G_p(p_1 - h G_p(p_0, q_1), q_1) \\\\\n",
    "    &= O(h),\n",
    "\\aa\n",
    "$\n",
    "\n",
    "thus,\n",
    "\n",
    "$\n",
    "G_p(p_0, q_1) + G_p(p_2, q_1)\n",
    "    = 2 G_p(p_1, q_1) +  h \\pp_p G_p(p_1, q_1) O(h) + O(h^2)\n",
    "    = 2 G_p(p_1, q_1) + O(h^2),\n",
    "$\n",
    "\n",
    "and,\n",
    "\n",
    "$\n",
    "p_2 - p_0 = h ( G_p(p_0, q_1) + G_p(p_2, q_1) ) = 2 h G_p(p_1, q_1) + O(h^3).\n",
    "$\n",
    "\n",
    "therefore,\n",
    "\n",
    "$\n",
    "x_2 - x_0 = 2 h G(x_1) + O(h^3).\n",
    "$\n",
    "\n",
    "Finllay, noting:\n",
    "\n",
    "$\n",
    "G(x_1) = G(x_0 + O(h^2)) = G(x_0) + O(h^2),\n",
    "$\n",
    "\n",
    "we have:\n",
    "\n",
    "$\n",
    "x_2 - x_0 = 2 h G(x_1) + O(h^3) = 2 h G(x_0) + O(h^3) = 2 h \\dot{x}_0 + O(h^3).\n",
    "$"
   ]
  },
  {
   "cell_type": "markdown",
   "metadata": {},
   "source": [
    "### Prop. 4.\n",
    "\n",
    "Assuming $G(p, q)$ is given by:\n",
    "\n",
    "- $G(p, q) = \\Mmp G_p(p, q) \\\\ G_q(p, q) \\mmp = \\Mmp B(q) \\\\ p \\mmp,$\n",
    "\n",
    "then, the sequence of pq-implicit method $p_0, p_1, p_2, p_3, p_4$ and $q_0, q_1, q_2, q_3, q_4$ satisfies:\n",
    "\n",
    "$\n",
    "\\Cc\\Aa\n",
    "q_2 &= q_0 + 2h p_0 + \\frac{(2h)^2}{2} B(q_0)  \\\\\n",
    "q_4 &= 2 q_2 - q_0 + (2h)^2 B(q_2)  \\\\\n",
    "p_2 &= \\frac{q_4 - q_0}{4 h}.\n",
    "\\aa\\cc\n",
    "$\n",
    "\n",
    "(aka. Verlet scheme by replacing $\\Delta_t = 2h$.)\n",
    "\n",
    "***Proof***"
   ]
  },
  {
   "cell_type": "markdown",
   "metadata": {},
   "source": [
    "For this special case, pq-implicit method gives:\n",
    "\n",
    "$\n",
    "\\Cc\\Aa\n",
    "p_1 &= p_0 + h B(q_0)  \\\\\n",
    "q_1 &= q_0 + h p_1     \\\\\n",
    "p_2 &= p_1 + h B(q_2)  \\\\\n",
    "q_2 &= q_1 + h p_1,\n",
    "\\aa\\cc\n",
    "$\n",
    "\n",
    "Here, we have:\n",
    "\n",
    "$\n",
    "\\Aa\n",
    "p_1 &= p_2 - h B(q_2)  \\\\\n",
    "p_3 &= p_2 + h B(q_2),\n",
    "\\aa\n",
    "$\n",
    "\n",
    "and:\n",
    "\n",
    "$\n",
    "\\Aa\n",
    "p_3 + p_1 &= 2 p_2 \\\\\n",
    "p_3 - p_1 &= 2 h B(q_2).\n",
    "\\aa\n",
    "$\n",
    "\n",
    "Also, we have:\n",
    "\n",
    "$\n",
    "\\Aa\n",
    "q_2 - q_0 &= 2 h p_1 \\\\\n",
    "q_4 - q_2 &= 2 h p_3.\n",
    "\\aa\n",
    "$\n",
    "\n",
    "Therfore:\n",
    "\n",
    "$\n",
    "\\Aa\n",
    "q_4 - 2 q_2 + q_0\n",
    "    &= (q_4 - q_2) - (q_2 - q_0)\n",
    "    =  2 h (p_3 - p_1)\n",
    "    =  (2 h)^2 B(q_2),\n",
    "\\aa\n",
    "$\n",
    "\n",
    "and:\n",
    "\n",
    "$\n",
    "\\Aa\n",
    "q_4 - q_0\n",
    "    &= (q_4 - q_2) + (q_2 - q_0)\n",
    "    =  2 h (p_3 + p_1)\n",
    "    =  4 h p_2,\n",
    "\\aa\n",
    "$\n",
    "\n",
    "and:\n",
    "\n",
    "$\n",
    "\\Aa\n",
    "q_2 - q_0\n",
    "    &= 2 h p_1\n",
    "    =  2 h p_0 + 4 h^2 B(q_0).\n",
    "\\aa\n",
    "$"
   ]
  }
 ],
 "metadata": {
  "kernelspec": {
   "display_name": "Python 3",
   "language": "python",
   "name": "python3"
  },
  "language_info": {
   "codemirror_mode": {
    "name": "ipython",
    "version": 3
   },
   "file_extension": ".py",
   "mimetype": "text/x-python",
   "name": "python",
   "nbconvert_exporter": "python",
   "pygments_lexer": "ipython3",
   "version": "3.8.2"
  }
 },
 "nbformat": 4,
 "nbformat_minor": 4
}
